theories/ml_lang/lang.v
@@ -781,12 +781,12 @@ Inductive prim_step p : expr → state → expr → state → Prop :=
   | Prim_step K e1 e2 σ1 σ2 e1' e2' :
     e1 = fill K e1' → e2 = fill K e2' →
     head_step p e1' σ1 e2' σ2 → prim_step p e1 σ1 e2 σ2
-  | Prim_step_raise K Ki e1 e2 σ1 σ2 v :
+  | Prim_step_raise K Ki e1 e2 σ1 v :
       e1 = fill (Ki :: K) (Raise (Val v)) → e2 = fill K (Raise (Val v)) →
-      ¬is_try Ki → prim_step p e1 σ1 e2 σ2
-  | Prim_step_try K e1 e2 σ1 σ2 r v :
+      ¬is_try Ki → prim_step p e1 σ1 e2 σ1
+  | Prim_step_try K e1 e2 σ1 r v :
       e1 = fill (TryCtx r :: K) (Raise (Val v)) → e2 = fill K (App r (Val v)) →
-      prim_step p e1 σ1 e2 σ2.
+      prim_step p e1 σ1 e2 σ1.
 
 (** External calls *)
 
@@ -878,9 +878,9 @@ Lemma prim_step_inv p e1 e2 σ1 σ2 :
   prim_step p e1 σ1 e2 σ2 →
   (∃ K e1' e2', e1 = fill K e1' ∧ e2 = fill K e2' ∧ head_step p e1' σ1 e2' σ2) ∨
   (∃ K Ki v, e1 = fill (Ki :: K) (Raise (Val v)) ∧
-             e2 = fill K (Raise (Val v)) ∧ ¬ is_try Ki) ∨
+             e2 = fill K (Raise (Val v)) ∧ ¬ is_try Ki ∧ σ1 = σ2) ∨
   (∃ K r v, e1 = fill (TryCtx r :: K) (Raise (Val v)) ∧
-            e2 = fill K (App r (Val v))).
+            e2 = fill K (App r (Val v)) ∧ σ1 = σ2).
 Proof.
   inversion 1; subst.
   { left; do 3 eexists; eauto. }
@@ -1147,8 +1147,8 @@ Local Lemma prim_step_fill p K e σ e' σ' :
   prim_step p (fill K e) σ (fill K e') σ'.
 Proof.
   intros [(K' & e1 & e2 & -> & -> & ?) |
-         [(K' & Ki & v  & -> & -> & ?) |
-          (K' & r  & v  & -> & ->)]]%prim_step_inv;
+         [(K' & Ki & v  & -> & -> & ? & ->) |
+          (K' & r  & v  & -> & -> & ->)]]%prim_step_inv;
   rewrite !fill_comp; by econstructor.
 Qed.
 
@@ -1194,8 +1194,8 @@ Local Lemma head_reducible_prim_step_ctx p K e1 σ1 e2 σ2 :
 Proof.
   intros (e2''&σ2''&HhstepK)
          [(K' & e1' & e2' & HKe1 & -> & Hstep) |
-         [(K' & Ki  & v   & HKe1 & -> & Ht) |
-          (K' & r   & v   & HKe1 & ->)]]%prim_step_inv.
+         [(K' & Ki  & v   & HKe1 & -> & Ht & ->) |
+          (K' & r   & v   & HKe1 & -> & ->)]]%prim_step_inv.
   { edestruct (step_by_outcome p K) as [K'' ?];
     eauto using outcome_head_stuck; simplify_eq/=.
     rewrite -fill_comp in HKe1; simplify_eq.
@@ -1278,8 +1278,8 @@ Local Lemma prim_step_call_dec p e σ e' σ' :
   (∃ fn vs K, is_call e fn vs K) ∨ (∀ fn vs K, ¬ is_call e fn vs K).
 Proof.
   intros [(K' & e1' & e2' & HKe1 & -> & Hstep) |
-         [(K' & Ki  & v   & HKe1 & -> & Ht) |
-          (K' & r   & v   & HKe1 & ->)]]%prim_step_inv; subst;
+         [(K' & Ki  & v   & HKe1 & -> & Ht & ->) |
+          (K' & r   & v   & HKe1 & -> & ->)]]%prim_step_inv; subst;
   try (right; intros fn vs K Hcall%eq_sym; now apply fill_call_raise in Hcall).
   destruct (to_outcome e1') eqn:Hval.
   { exfalso. apply outcome_head_stuck in Hstep. congruence. }
@@ -1309,15 +1309,14 @@ Local Lemma prim_step_no_call p1 p2 e σ e' σ' :
 Proof.
   intros Hncall.
   intros [(K' & e1' & e2' & HKe1 & -> & Hstep) |
-         [(K' & Ki  & v   & HKe1 & -> & Ht) |
-          (K' & r   & v   & HKe1 & ->)]]%prim_step_inv; subst.
+         [(K' & Ki  & v   & HKe1 & -> & Ht & ->) |
+          (K' & r   & v   & HKe1 & -> & ->)]]%prim_step_inv; subst.
   { inversion Hstep; subst.
     all: try repeat (econstructor; eauto).
     exfalso. eapply Hncall. done. }
-  { apply (Prim_step_raise p2 K' Ki _ _ _ _ v); eauto. }
-  { apply (Prim_step_try p2 K' _ _ _ _ r v); eauto. }
+  { apply (Prim_step_raise p2 K' Ki _ _ _ v); eauto. }
+  { apply (Prim_step_try p2 K' _ _ _ r v); eauto. }
 Qed.
-(* Qed. *)
 
 End ML_lang.
 Export ML_lang.
