theories/interop/wp_prims/raise.v
@@ -1,0 +1,49 @@
+From iris.proofmode Require Import proofmode.
+From transfinite.base_logic.lib Require Import ghost_map ghost_var.
+From melocoton Require Import named_props stdpp_extra.
+From melocoton.mlanguage Require Import mlanguage.
+From melocoton.c_interface Require Import defs notation resources.
+From melocoton.interop Require Import state lang basics_resources.
+From melocoton.interop Require Import basics wp_utils.
+From melocoton.interop Require Export prims weakestpre prims_proto.
+From melocoton.interop.wp_prims Require Import common.
+From melocoton.mlanguage Require Import weakestpre.
+Import Wrap.
+
+Section Laws.
+
+Context `{SI: indexT}.
+Context {Σ : gFunctors}.
+Context `{!heapG_ML Σ, !heapG_C Σ}.
+Context `{!invG Σ}.
+Context `{!wrapperG Σ}.
+
+Implicit Types P : iProp Σ.
+Import mlanguage.
+
+Lemma raise_correct e : |- wrap_prog e :: raise_proto.
+Proof using.
+  iIntros (Hnprim ? ? ?) "Hproto". iNamedProto "Hproto".
+  iSplit; first done. iIntros (Φ'') "Hb Hcont".
+  iApply wp_wrap_call; first done. cbn [snd].
+
+  rewrite weakestpre.wp_unfold. rewrite /weakestpre.wp_pre.
+  iIntros (σ) "Hst".
+  iDestruct (SI_at_boundary_is_in_C with "Hst Hb") as %(ρc&mem&->). simpl.
+
+  iModIntro.
+  iRight; iRight. iSplit; first done.
+  iExists (λ '(e2, σ2),
+    e2 = WrSE (ExprO (OExn w)) ∧
+    σ2 = CState ρc mem).
+  iSplit. { iPureIntro. eapply PrimS. eapply RaiseS; eauto. }
+  iIntros (? ? (-> & ->)).
+  do 3 iModIntro. iFrame "Hst".
+  rewrite weakestpre.wp_unfold. rewrite /weakestpre.wp_pre.
+  iIntros (σ) "Hst".
+  iModIntro. iLeft. iExists (OExn w). cbn. iFrame. iSplit; first done.
+  iApply "Hcont". iFrame.
+  iApply "Cont". iFrame.
+Qed.
+
+End Laws.
