theories/interop/wp_simulation_catch.v
@@ -10,11 +10,11 @@ From iris.proofmode Require Import proofmode.
 From melocoton.c_interface Require Import defs resources.
 From melocoton.ml_lang Require Import lang lang_instantiation primitive_laws proofmode.
 From melocoton.interop Require Export prims weakestpre prims_proto hybrid_ghost_heap.
-From melocoton.interop Require Import wp_ext_call_laws wp_boundary_laws wp_utils wp_simulation_catch.
+From melocoton.interop Require Import wp_ext_call_laws wp_boundary_laws wp_utils.
 From melocoton.interop.wp_prims Require Import common.
 Import Wrap.
 
-Section Simulation.
+Section Simulation_catch.
 
 Context `{SI: indexT}.
 Context {Σ : gFunctors}.
@@ -27,12 +27,20 @@ Import mlanguage.
 
 Local Notation CValI n := (C_intf.LitV (C_intf.LitInt n)).
 Local Notation CValL a := (C_intf.LitV (C_intf.LitLoc a)).
+Local Notation HVal v := (Some (Some v)).
 
-Lemma wp_to_outcome (pe : progenv.prog_environ wrap_lang Σ) (o : outcome MLval):
+Lemma wp_to_outcome_catch (pe : progenv.prog_environ wrap_lang Σ) (o : outcome MLval):
   not_at_boundary
- -∗ WP (WrSE (ExprML (language.of_outcome ML_lang o) false)) at pe {{ ret,
-   ∃ θ' olv, GC θ' ∗ ⌜repr_lval_out θ' olv ret⌝ ∗
-             olv ~~ₒ o ∗ at_boundary wrap_lang }}.
+ -∗ WP (WrSE (ExprML (language.of_outcome ML_lang o) true)) at pe {{ ret,
+   ∃ θ' exn lv a w,
+     ⌜ret = OVal (CValL a)⌝ ∗
+     a ↦C∗ [exn; w] ∗
+     GC θ' ∗
+     match o with
+     | OVal v => ⌜exn = CValI 0⌝ ∗ ⌜repr_lval θ' lv w⌝ ∗ lv ~~ v
+     | OExn v => ⌜exn = CValI 1⌝ ∗ ⌜repr_lval θ' lv w⌝ ∗ lv ~~ v
+     end ∗
+     at_boundary wrap_lang }}.
 Proof using.
   iIntros "Hnb".
   rewrite weakestpre.wp_unfold. rewrite /weakestpre.wp_pre.
@@ -51,26 +59,77 @@ Proof using.
   iExists (λ '(e', σ'), ∃ ow ρc mem,
     ml_to_c_heap ρml σ ρc mem ∧
     ml_to_c_outcome o ow ρc ∧
-    e' = WrSE (ExprO (ow)) ∧ σ' = CState ρc mem).
+    e' = WrSE (ExprOC (ow)) ∧ σ' = CState ρc mem).
   iSplit.
   { iPureIntro. eapply OutS; try naive_solver.
     apply language.to_of_outcome. }
 
   iIntros (? ? (w & ρc & mem & Hout & Hcore & -> & ->)).
-  iMod (wrap_interp_ml_to_c_out with "SI Hnb") as "(SI & Hb & HGC & (%ov & Hbo & %Hrepr))";
+  iMod (wrap_interp_ml_to_c_out with "SI Hnb") as "(SI & Hb & HGC & H)";
     first done; first done.
   do 3 iModIntro. iFrame "SI".
+
+  rewrite weakestpre.wp_unfold. rewrite /weakestpre.wp_pre.
+  iIntros "%st SI".
+  iDestruct (SI_at_boundary_is_in_C with "SI Hb") as "%H"; destruct H as (ρc' & σ' & ->).
+  iModIntro. iRight. iRight.
+  iSplit; first done.
+
+  pose (match w with OVal _ => 0 | OExn _ => 1 end) as is_exn.
+  pose (match w with OVal v | OExn v => v end) as ov.
+
+  iExists (λ '(e'', σ''), ∃ a nmem,
+    σ' !! a = None ∧
+    σ' !! (a +ₗ 1) = None ∧
+    nmem = heap_array a [HVal (CValI is_exn); HVal ov] ∪ σ' ∧
+    e'' = WrSE (ExprO (OVal (CValL a))) ∧
+    σ'' = CState ρc' (heap_array a [HVal (CValI is_exn); HVal ov] ∪ σ')).
+  iSplit.
+  { iPureIntro. eapply RetCS; intros. eexists a, _; split_and!; eauto.
+    destruct w; subst; eauto. }
+
+  iIntros (? ? (a & nmem' & Ha & Ha1 & -> & -> & ->)). do 2 iModIntro.
+  iDestruct "SI" as "[HσC SIC]".
+  iMod (gen_heap_alloc_big σ' (heap_array a [HVal (CValI is_exn); HVal ov]) with "[HσC]")
+    as "(Hσ & Hl & Hm)"; eauto.
+  { apply heap_array_map_disjoint; cbn. intros i Hi0 Hil.
+    assert (i = 0 ∨ i = 1) as [-> | ->] by lia; eauto. now rewrite loc_add_0. }
+  iModIntro. iFrame.
+
   iApply weakestpre.wp_outcome'.
-  iExists _, _. iFrame. by inversion Hrepr; simplify_eq.
+  iDestruct "H" as "(%olv & Hls & %Hval)". cbn.
+  rewrite big_opM_union; last first.
+  { apply map_disjoint_spec=> l' v1 v2 /lookup_singleton_Some [-> _].
+    intros H. rewrite lookup_union_r in H.
+    { rewrite lookup_empty in H. congruence. }
+    rewrite insert_empty. apply lookup_singleton_ne. destruct l'.
+    inversion 1. lia. }
+  iDestruct "Hl" as "[Ha1 Ha2]".
+  rewrite big_opM_union; last first.
+  { apply map_disjoint_spec=> l' v1 v2 /lookup_singleton_Some. intros [<- H'].
+    rewrite lookup_empty. congruence. }
+  iDestruct "Ha2" as "[Ha2 _]".
+  destruct o; destruct olv; try iDestruct "Hls" as "%H";
+  try (now inversion H);
+  inversion Hval; subst;
+  iExists _, _, _, _, _; iFrame; repeat (iSplit; eauto).
+  all: iSplitR "Ha2"; try rewrite loc_add_0; rewrite big_opM_singleton; eauto.
 Qed.
 
-Lemma wp_simulates (Ψ : protocol ML_lang.val Σ) eml emain Φ :
+Lemma wp_simulates_catch (Ψ : protocol ML_lang.val Σ) eml emain Φ :
   Ψ on prim_names ⊑ ⊥ →
   not_at_boundary -∗
   WP eml at ⟨ ∅, Ψ ⟩ {{ Φ }} -∗
-  WP (WrSE (ExprML eml false)) at ⟪ wrap_prog emain, wrap_proto Ψ ⟫ {{ o,
-    ∃ θ' ov olv, GC θ' ∗ ⌜repr_lval_out θ' olv o⌝ ∗ olv ~~ₒ ov ∗ Φ ov ∗
-    at_boundary wrap_lang }}.
+  WP (WrSE (ExprML eml true)) at ⟪ wrap_prog emain, wrap_proto Ψ ⟫
+  {{ o, ∃ θ' res is_exn ret lret wret,
+    ⌜o = OVal (C_intf.LitV (C_intf.LitLoc res))⌝ ∗
+    GC θ' ∗
+    res ↦C∗ [ C_intf.LitV (C_intf.LitInt is_exn); wret ] ∗
+    lret ~~ ret ∗ ⌜repr_lval θ' lret wret⌝ ∗
+    at_boundary wrap_lang ∗
+    if Z.eqb is_exn 0%Z
+    then Φ (OVal ret)
+    else Φ (OExn ret) }}.
 Proof.
   intros Hnprims.
   iLöb as "IH" forall (eml).
@@ -83,15 +142,19 @@ Proof.
   iMod ("HWP" $! σ with "[$HσML]") as "[HWP|[HWP|HWP]]".
   (* value *)
   + iDestruct "HWP" as "(%o & -> & Hσ & Hret)".
-    iPoseProof (wp_to_outcome _ o with "Hnb") as "Hwp".
+    iPoseProof (wp_to_outcome_catch _ o with "Hnb") as "Hwp".
     iDestruct (weakestpre.wp_strong_mono_post with "[Hret] Hwp") as "Hwp";
       last first.
     { rewrite weakestpre.wp_unfold. rewrite /weakestpre.wp_pre.
       iApply ("Hwp" $! (MLState ρml σ)). iFrame. by iPureIntro. }
-    { cbn. iIntros (vv) "(%θ' & %olv & HGC & %Hrep & Hval & ?)".
-      iExists _, _, _. iFrame. eauto. }
+    { iIntros (vv) "(%θ' & %exn & %lv & %a & %w & -> & Ha & HGC & H & ?)".
+      destruct o.
+      { iExists θ', a, _, _, _, _. iFrame.
+        iDestruct "H" as "(-> & %Hr & Hb)". iFrame; iSplit; eauto.  }
+      { iExists θ', a, _, _, _, _. iFrame.
+        iDestruct "H" as "(-> & %Hr & Hb)". iFrame; iSplit; eauto.  } }
   (* extcall *)
-  + iDestruct "HWP" as "(%fn_name & %vs & %K' & -> & %Hfn & >(%Ξ & Hσ & HT & Hr))".
+  + iDestruct "HWP" as "(%fn_name & %vs & %K' & %H & %Hfn & >(%Ξ & Hσ & HT & Hr))".
     iAssert (⌜¬ is_prim_name fn_name⌝)%I with "[HT]" as "%Hnprim".
     { destruct (decide (is_prim_name fn_name)) as [His|]; last by eauto.
       cbn -[wrap_prog]. iDestruct (Hnprims with "[HT]") as "%"; last done.
@@ -107,17 +170,16 @@ Proof.
       Forall2 (is_val (χC ρc) (ζC ρc)) vs lvs ∧
       Forall2 (repr_lval (θC ρc)) lvs ws ∧
       ml_to_c_heap ρml σ ρc mem ∧
-      e' = WrE (Wrap.ExprCall fn_name ws) [(K', false)] ∧
+      e' = WrE (Wrap.ExprCall fn_name ws) [(K', true)] ∧
       σ' = CState ρc mem).
     iSplit.
     { iPureIntro.
       eapply MakeCallS; eauto.
-      { done. }
       { apply not_elem_of_dom. rewrite dom_wrap_prog not_elem_of_prim_names //. }
       { split_and!; eauto. }
       { intros * Hep (lvs & ? & ?). do 4 eexists. split_and!; eauto. } }
     iIntros (? ? (ws & ρc & mem & lvs & ? & ? & Hcore & -> & ->)).
-    iMod ((wrap_interp_ml_to_c vs lvs) with "[- Hnb Hr HT] Hnb")
+    iMod ((wrap_interp_ml_to_c vs lvs _ _ ws) with "[- Hnb Hr HT] Hnb")
       as "(Hσ & Hb & HGC & (#Hblk & %))"; eauto.
     { rewrite /wrap_state_interp /ML_state_interp /named.
       iSplitL "Hσ"; first by iFrame. by iFrame. }
@@ -129,7 +191,7 @@ Proof.
     iIntros (st') "Hst'".
     iDestruct (SI_at_boundary_is_in_C with "Hst' Hb") as %(ρc'&mem'&->).
 
-    iModIntro. iRight; iLeft. iExists fn_name, ws, [(K', false)].
+    iModIntro. iRight; iLeft. iExists fn_name, ws, [(K', true)].
     iSplit; first done.
     iSplit.
     { iPureIntro. apply not_elem_of_dom.
@@ -152,15 +214,13 @@ Proof.
     iDestruct ((wrap_interp_c_to_ml_out wret _ _ _ vret lvret) with "Hst' HGC Hb [Hsim]")
       as (ρml' σ' ζ Hc_to_ml_heap Hc_to_ml_out) "HH"; eauto.
     iExists (λ '(e2, σ2),
-      e2 = WrSE (ExprML (language.fill K' (lang.ML_lang.of_outcome vret)) false) ∧
+      e2 = WrSE (ExprML (language.fill K' (lang.ML_lang.of_outcome vret)) true) ∧
       σ2 = MLState ρml' σ').
-    iSplit.
-    { iPureIntro. eapply RetS; eauto. }
+    iSplit. { iPureIntro. eapply RetS; eauto. }
     iIntros (? ? (-> & ->)). iMod "HH" as "[Hst' Hnb]".
     do 3 iModIntro. iFrame "Hst'".
 
     (* continue execution using IH *)
-
     iApply ("IH" with "Hnb").
     by iApply "Hr".
 
@@ -169,7 +229,7 @@ Proof.
     iModIntro. iRight. iRight. iSplit; first done.
     iExists (λ '(e2, σ2), ∃ eml' σ',
       language.language.prim_step ∅ eml σ eml' σ' ∧
-      e2 = WrSE (ExprML eml' false) ∧ σ2 = MLState ρml σ').
+      e2 = WrSE (ExprML eml' true) ∧ σ2 = MLState ρml σ').
     iSplit.
     { iPureIntro. eapply StepMLS; eauto.
       by eapply reducible_not_val. }
@@ -182,9 +242,9 @@ Proof.
     iApply ("IH" with "Hnb HWP'").
 Qed.
 
-Lemma callback_correct emain Ψ :
+Lemma callback_exn_correct emain Ψ :
   Ψ on prim_names ⊑ ⊥ →
-  wrap_proto Ψ |- wrap_prog emain :: callback_proto Ψ.
+  wrap_proto Ψ |- wrap_prog emain :: callback_exn_proto Ψ.
 Proof using.
   iIntros (Hnprim ? ? ?) "Hproto". iNamedProto "Hproto".
   iSplit; first done. iIntros (Φ'') "Hb Hcont".
@@ -213,83 +273,17 @@ Proof using.
   iModIntro.
   iRight; iRight. iSplit; first done.
   iExists (λ '(e2, σ2),
-    e2 = WrSE (ExprML (App (Val (RecV f x e)) (Val v')) false) ∧
+    e2 = WrSE (ExprML (App (Val (RecV f x e)) (Val v')) true) ∧
     σ2 = MLState ρml' σ').
-  iSplit. { iPureIntro. eapply CallbackS; eauto. }
+  iSplit. { iPureIntro. eapply CallbackexnS; eauto. }
   iIntros (? ? (-> & ->)). iMod "HH" as "(Hst & Hnb)".
   do 3 iModIntro. iFrame "Hst".
   iApply (weakestpre.wp_wand with "[-Cont Hcont Hclos]").
-  { by iApply (wp_simulates with "Hnb [WPcallback]"). }
-  cbn. iIntros (o) "(%θ' & %lv & %vret & HGC & % & Hsim & Hψ & ?)".
+  { iApply (wp_simulates_catch with "Hnb [WPcallback]"); eauto. }
+  cbn. iIntros (o) "(%θ' & %res & %is_exn & %ret & %lret & %wret & -> & HGC & H)".
+  iDestruct "H" as "((Hexn & Hres & _) & Hb & Hr & ? & H)".
   iApply "Hcont". iFrame.
   iApply "Cont". iFrame; eauto.
 Qed.
 
-Lemma main_correct emain Ψ P (Φ : Z → Prop) :
-  Ψ on prim_names ⊑ ⊥ →
-  (⊢ P -∗ WP emain at ⟨∅, Ψ⟩ {{ k, ⌜∃ x, k = OVal (LitV (LitInt x)) ∧ Φ x⌝ }}) →
-  wrap_proto Ψ |- wrap_prog emain :: main_proto Φ P.
-Proof using.
-  iIntros (Hnprim Hmain ? ? ?) "Hproto". iNamedProto "Hproto".
-  iSplit; first done. iIntros (Φ') "Hb Hcont".
-  iApply wp_wrap_call; first done. cbn [snd].
-  rewrite weakestpre.wp_unfold. rewrite /weakestpre.wp_pre.
-  iIntros (st) "Hst".
-  iDestruct (SI_at_boundary_is_in_C with "Hst Hb") as %(ρc&mem&->). simpl.
-  iNamed "Hst". iNamed "SIC". unfold gctoken.at_init.
-  iDestruct (ghost_var_agree with "Hat_init SIinit") as %?; simplify_eq.
-  iNamed "Hinit". iRename "Hat_init" into "GCinit".
-  destruct ρc. cbn [state.ζC state.χC state.θC state.rootsC] in *. SI_GC_agree.
-  iAssert (ghost_var wrapperG_γat_init 1 true) with "[GCinit SIinit]" as "SIinit".
-  { rewrite -{3}Qp.half_half.
-    iApply (fractional.fractional_merge _ _ (λ q, ghost_var wrapperG_γat_init q true)
-             with "GCinit SIinit"). }
-  iMod (ghost_var_update false with "SIinit") as "SIinit".
-  iMod (ghost_var_update_halves false with "Hb SIbound") as "[Hb SIbound]".
-
-  iModIntro.
-  iRight; iRight. iSplit; first done.
-  iExists (λ '(e2, σ2),
-    e2 = WrSE (ExprML emain false) ∧
-    σ2 = MLState {| χML := ∅; ζML := ∅; rootsML := ∅ |} ∅).
-  iSplit. { iPureIntro. eapply MainS; eauto. }
-  iIntros (? ? (-> & ->)).
-  do 3 iModIntro.
-
-  rewrite [X in ghost_var wrapperG_γat_init X _](_: 1 = 1/2 + 1/2)%Qp;
-    last by rewrite Qp.half_half.
-  iDestruct (ghost_var_split _ _ (1/2) (1/2) with "SIinit") as "[Hinit1 Hinit2]".
-  rewrite /weakestpre.state_interp /= /named.
-  rewrite /ML_state_interp /= /named.
-  rewrite /public_state_interp.
-  rewrite !fmap_empty !right_id_L !dom_empty_L. iFrame.
-  rewrite /named !dom_empty_L big_sepS_empty. iFrame.
-  iSplitL "GCζvirt GCχvirt". { iSplit; eauto. iApply (hgh_empty with "[$] [$]"). }
-
-  iApply (weakestpre.wp_wand with "[-Cont Hcont]").
-  { iApply (wp_simulates with "Hb [Hinitial_resources]"); first done.
-    iApply (Hmain with "[$]"). }
-  cbn. iIntros (o) "(%θ' & %v & %lv & HGC & %Hrepr & Hsim & HΦ' & ?)".
-  iDestruct "HΦ'" as (?) "[%Hv %HΦ]". inversion Hv. subst.
-  destruct lv.
-  { iDestruct "Hsim" as "->". inversion Hrepr; simplify_eq.
-    inversion H2; simplify_eq.
-    iApply "Hcont". iFrame. by iApply "Cont". }
-  { iDestruct "Hsim" as "%Hf". inversion Hf.  }
-Qed.
-
-Lemma wrap_correct emain Ψ (Φ : Z → Prop) P :
-  Ψ on prim_names ⊑ ⊥ →
-  (⊢ P -∗ WP emain at ⟨∅, Ψ⟩ {{ k, ⌜∃ x, k = OVal (LitV (LitInt x)) ∧ Φ x⌝ }}) →
-  wrap_proto Ψ |- wrap_prog emain :: prims_proto Ψ ⊔ main_proto Φ P.
-Proof using.
-  intros Hnprim Hmain.
-  iIntros (? ? ?) "[Hprim|Hmain]".
-  { iDestruct "Hprim" as (p) "H".
-    destruct p; last (by iExFalso); try by iApply (base_prim_correct with "H").
-    { by iApply (callback_exn_correct with "H"). }
-    { by iApply (callback_correct with "H"). } }
-  { by iApply (main_correct with "Hmain"). }
-Qed.
-
-End Simulation.
+End Simulation_catch.
